AbsInterp/Framework/Iteration.lean
@@ -1,3 +1,4 @@
 import AbsInterp.Framework.Iteration.NatIter
 import AbsInterp.Framework.Iteration.Collecting
+import AbsInterp.Framework.Iteration.Fixpoint
 import AbsInterp.Framework.Iteration.Widening
